\documentclass[]{article}
\usepackage{amsmath,amssymb,amsthm}
\usepackage[utf8]{inputenc}
\usepackage{lmodern}
%\usepackage{circuitikz}
\makeatletter
\@ifpackageloaded{tex4ht}{
    \def\pgfsysdriver{pgfsys-tex4ht.def}
}
\makeatother
\usepackage{pgfplots}
\usepackage{pgfplotstable}
\usepackage{pgf,tikz}
\usetikzlibrary{shapes,backgrounds,positioning,matrix,decorations}

\usepackage{siunitx}
\usepackage{python}
\usepackage{ifxetex,ifluatex}
\usepackage{listings}
\setlength{\parskip}{3mm}
\newtheorem{axiom}{Axiom}
\newtheorem{definition}{Definition}
\newtheorem{comment}{Comment}
\newtheorem{example}{Example}
\newtheorem{lemma}{Lemma}
\newtheorem{property}{Property}
\newtheorem{problem}{Problem}
\newtheorem{remark}{Remark}
\newtheorem{theorem}{Theorem}
\newtheorem{script}{Script}

\usepackage{fixltx2e} % provides \textsubscript
% use upquote if available, for straight quotes in verbatim environments
\IfFileExists{upquote.sty}{\usepackage{upquote}}{}
\ifnum 0\ifxetex 1\fi\ifluatex 1\fi=0 % if pdftex
  \usepackage[utf8]{inputenc}
\else % if luatex or xelatex
  \ifxetex
    \usepackage{mathspec}
    \usepackage{xltxtra,xunicode}
  \else
    \usepackage{fontspec}
  \fi
  \defaultfontfeatures{Mapping=tex-text,Scale=MatchLowercase}
  \newcommand{\euro}{â‚¬}
\fi
% use microtype if available
\IfFileExists{microtype.sty}{\usepackage{microtype}}{}
\ifxetex
  \usepackage[setpagesize=false, % page size defined by xetex
              unicode=false, % unicode breaks when used with xetex
              xetex]{hyperref}
\else
  \usepackage[unicode=true]{hyperref}
\fi
\hypersetup{breaklinks=true,
            bookmarks=true,
            pdfauthor={Neetu Saini},
            pdftitle={Cold Denaturation},
            colorlinks=true,
            citecolor=blue,
            urlcolor=blue,
            linkcolor=magenta,
            pdfborder={0 0 0}}
\urlstyle{same}  % don't use monospace font for urls
\setlength{\parindent}{0pt}
\setlength{\parskip}{6pt plus 2pt minus 1pt}
\setlength{\emergencystretch}{3em}  % prevent overfull lines
\setcounter{secnumdepth}{0}

\title{Cold Denaturation}
\author{Neetu Saini \footnote{Typesetting by Dilawar Singh}}
\date{}
\usepackage[margin=15mm]{geometry}

\begin{document}
\maketitle

\section{Starting equations.}\label{starting-equations.}

\begin{subequations}
    \begin{align}
        \Delta H &= \Delta H^0 + \Delta C_P (T - T_0) \label{eq:enthalpy} \\
        \Delta S &= \Delta S^0 + \Delta C_P \ln{\frac{T}{T_0}} \label{eq:entropy}
    \end{align}
\end{subequations}

\begin{equation}
    \Delta G = \Delta H - T \Delta S \label{eq:gibbs}
\end{equation}

We put equations \ref{eq:enthalpy} and \ref{eq:entropy} into equation
\ref{eq:gibbs} and we get the following.

\begin{align}
    \Delta G &= \Delta H^0 + \Delta C_P (T - T_0) - T \times \left(\Delta S^0 + \Delta C_P \ln{\frac{T}{T_0}}\right) \\
     &= \left(\Delta H^0 - T\Delta S^0 \right) + \Delta C_P (T - T_0) - T \Delta C_P \ln{\frac{T}{T_0}} \label{eq:gibbs1}
\end{align}

where $T_0$ is any reference temperature.

\section{Equation \ref{eq:gibbs1} at $T_g$ and
$T'_g$}\label{equation-at-tux5fg-and-tux5fg}

\textbf{At temperature $Tg$ and $T'_g$ $\Delta G$ in equations
\ref{eq:gibbs} goes to 0}

\begin{subequations}
    \label{eq:subequation}
    \begin{align}
        \Delta H(T_g) = T_g \Delta S(T_g) \label{eq:enthalpy0} \\
        \Delta H(T'_g) = T'_g \Delta S(T'_g) \label{eq:enthalpy1} 
    \end{align}
\end{subequations}

In equation \ref{eq:gibbs1}, we choose reference temperature are $T_g$
and compute $\Delta G$ at $T'_g$ which is 0.

\begin{align}
    0 = \Delta G(T'_g) &= \Delta H(T_g) - T'_g \Delta S(T_g) + \Delta C_P (T'_g -
        T_g) - T'_g \Delta C_P \ln{\frac{T'_g}{T_g}}  \\
        &= \Delta H(T_g) - T'_g \frac{\Delta H(T_g)}{T_g} + \Delta C_P (T'_g -
        T_g) - T'_g \Delta C_P \ln{\frac{T'_g}{T_g}} && \mbox{substituting
    \ref{eq:enthalpy0}}  \\
    &= \Delta H(T_g) \left(1 - \frac{T'_g}{T_g} \right) + \Delta C_P (T'_g -
        T_g) - T'_g \Delta C_P \ln{\frac{T'_g}{T_g}} \\
    &= \Delta H(T_g) \left(\frac{T_g - T'_g}{T_g} \right) + \Delta C_P (T'_g -
        T_g) - T'_g \Delta C_P \ln{\frac{T'_g}{T_g}} \\
\end{align}

$\implies$

\begin{align}
    - \frac{\Delta H(T_g)}{\Delta C_P} \left(\frac{T_g - T'_g}{T_g} \right) 
    &= T'_g - T_g - T'_g \ln{\frac{T'_g}{T_g}} \\
    &= T'_g - T_g + T'_g \ln{\frac{T_g}{T'_g}} \\
    &= T'_g - T_g + T'_g \ln\left(1+{\frac{T_g - T'_g}{T'_g}}\right) && \mbox{$x = 1 + x - 1$} \\
    &= T'_g - T_g + T'_g \left({\frac{T_g - T'_g}{T'_g}} - \frac{1}{2}\left(
    \frac{T_g - T'_g}{T'_g} \right)^2 \right) && \mbox{$\ln(1+x) = x -
\frac{x^2}{2} \ldots $} \\
&= T'_g - T_g + T_g - T'_g - \frac{T'_g}{2} \left( \frac{T_g - T'_g}{T'_g}
\right)^2  \\
\implies  - \frac{\Delta H(T_g)}{\Delta C_P} \left(\frac{T_g - T'_g}{T_g} \right)
    &= - \frac{T'_g}{2} \left( \frac{T_g - T'_g}{T'_g} \right)^2 \\
 \frac{\Delta H(T_g)}{\Delta C_P} &=  \frac{T'_gT_g}{2} \left( \frac{T_g - T'_g}{T'_g} \right)^2 \\ 
 \frac{2\Delta H(T_g)}{\Delta C_P} &=  T_g \frac{T_g - T'_g}{T'_g} \\ 
\frac{2\Delta H(T_g)}{\Delta C_P} &=   \frac{T_g^2}{T'_g} - T_g \\ 
\frac{2\Delta H(T_g)}{\Delta C_P} + T_g &=   \frac{T_g^2}{T'_g}  
\end{align}

\begin{equation}
    \boxed{T'_g = \frac{T_g^2}{\frac{2\Delta H(T_g)}{\Delta C_P} + T_g}}
\end{equation}

\end{document}
